SeLe4n/Kernel/API.lean
@@ -10,3 +10,5 @@ import SeLe4n.Kernel.Service.Operations
 import SeLe4n.Kernel.Service.Invariant
 
 import SeLe4n.Kernel.Architecture.Assumptions
+
+import SeLe4n.Kernel.Architecture.Adapter
